## $\lambda$-calculus

### $\beta$-reduction

$$
(\lambda x \ . \ e) \ . \ e' \overset{\beta}\rightarrow e[x \rightarrow e']
$$

### $\alpha$-reduction

$$
\lambda x \ . \ e \overset{\alpha}\rightarrow \lambda y \ . \ e
$$

### First-class Functions

> **Note**: first-class means that functions can be treated like any other value.

$$
\begin{aligned}
&\ \left(\left(\lambda x \cdot (\lambda y \cdot x) z\right)\right) 9
\end{aligned}
$$

#### Example

$$
\begin{aligned}
  &\ (((\lambda f \ . \ (\lambda y \ . \ (f (f(y))) (\lambda x \ . \ x \cdot x)) 3) \\
= &\ (((\lambda y \ . \ ((\lambda x \ . \ x \cdot x) ((\lambda x \ . \ x \cdot x)(y))) 3) \\
= &\ (\lambda x \ . \ x \cdot x) ((\lambda x \ . \ x \cdot x) \cdot 3) \\
= &\ (\lambda x \ . \ x \cdot x) (3 \cdot 3) \\
= &\ (3 \cdot 3) \cdot (3 \cdot 3) \\
= &\ 81
\end{aligned}
$$

#### Functions with Multiple Arguments

$$
\begin{aligned}
&\ \lambda x, y \ . \ x + y \\
\equiv &\ \lambda x \ . \ (\lambda y \ . \ x+y) \ \ \ \text{(currying)} \\
\end{aligned}
$$

```js
// (y) => f is a closure! It captures x from the outer scope.
const addn = (x) => (y) => x + y;
const add3 = addn(3);
add3(4); // 7
```

### Enhanced $\lambda$-calculus

Includes:

- Booleans

  Implementation:

  $$
  T \equiv \lambda x \ . \ \lambda y \ . \ x \\
  F \equiv \lambda x \ . \ \lambda y \ . \ y \\
  IF
  $$

- Numbers and numeric operations
- Ifs
- Lists $<e_1, e_2, ..., e_n>$

  - Head $a$
  - Tail $<b, c, ..., n>$
  - Pairs $<a, b>$

  $$
  <e_1, <e_2, < ... <e_n, \perp> ... > > >
  $$

  Implementation:

  $$
  \begin{aligned}
  \text{PAIR}(1, 2) &\approx (\lambda g \ . \ g \ 1 \ 2) \\
  \text{HEAD} &\equiv \lambda a, b \ . \ a \\
  \text{TAIL} &\equiv \lambda a, b \ . \ b \\
  \end{aligned}
  $$

  Example:

  $$
  \begin{aligned}
  &\ \text{HEAD}(\text{PAIR}(1, 2)) \\
  &\ \text{HEAD}(\lambda g \ . \ g \ 1 \ 2) \\
  &\ (\lambda a, b \ . \ a \ 1 \ 2) (\lambda g \ . \ g \ 1 \ 2) \\
  &\ (\lambda a, b \ . \ a) \ 1 \ 2 \\
  &\ 1
  \end{aligned}
  $$

- Map, Reduce, Filter
- Recursion

  $$
  \begin{aligned}
  F&(\text{self}, x) \ \text{self}(x - 1) \\
  f& = \text{RECURSE} \ F
  \end{aligned}
  $$
